src/Serial.v
@@ -1,42 +1,45 @@
 Require Import Bool List String Peano_dec.
-Require Import Common FMap Syntax Semantics StepDet.
+Require Import Common ListSupport FMap Syntax Semantics StepDet.
 
 (** [Atomic] and [Transactional] histories *)
 
 Section PerSystem.
   Variable sys: System.
 
-  (* Note that due to the definition of [TMsg], it is guaranteed that an
-   * [Atomic] history is about a single transaction. [TMsg] contains
-   * [tmsg_tid], and [In hdl mouts] in [AtomicCons] ensures that the history is
-   * for a single transaction.
+  (* A history is [Atomic] if it satisfies the following conditions:
+   * 0) The history can be either an incomplete or a complete transaction. 
+   * 1) Each label in the history has a form of [IlblOuts (Some hdl) _],
+   *    and all [hdl]s have the same [tinfo_tid]. It means that the history is
+   *    for a single transaction.
+   * 2) No external output messages are generated until the transaction ends.
+   *    (Reflected in [AtomicCont])
+   * 3) When the transaction ends, it outputs a single external message, which
+   *    is the response of the original request.
+   *    (Reflected in [AtomicFin])
+   * 4) When the transaction ends, no internal messages about the transaction 
+   *    are left. We ensure it by just tracking the internal messages about
+   *    the transaction ([mouts]).
    *)
   Inductive Atomic: TInfo -> History -> MessagePool TMsg -> option TMsg -> Prop :=
-  | AtomicStart:
-      forall tid rqin tinfo,
-        isExternal sys (mid_from (msg_id (getMsg rqin))) = true ->
-        tinfo = {| tinfo_tid := tid; tinfo_rqin := rqin |} ->
-        Atomic tinfo nil (enqMP (toTMsg tinfo rqin) nil) None
-  | AtomicCont:
-      forall rqin hst mouts,
-        Atomic rqin hst mouts None ->
-        forall hdl houts,
-          InMP hdl mouts ->
-          isInternal sys (mid_from (msg_id (tmsg_msg hdl))) = true ->
-          ForallMP (fun tmsg => isInternal sys (mid_to (msg_id (tmsg_msg tmsg))) = true) houts ->
-          (* When coupled with [steps_det], we can prove that
-           * [deqMP from to chn mouts] dequeues [hdl].
-           *)
-          forall from to chn,
-            firstMP from to chn mouts = Some hdl ->
-            Atomic rqin (IlblOuts (Some hdl) houts :: hst)
-                   (distributeMsgs houts (deqMP from to chn mouts)) None
-  | AtomicFin:
-      forall rqin hst hdl rsout,
-        Atomic rqin hst (hdl :: nil) None ->
-        isInternal sys (mid_from (msg_id (tmsg_msg hdl))) = true ->
+  | AtomicImm:
+      forall tid (rqin: Msg) rsout,
+        isExternal sys (mid_from (msg_id rqin)) = true ->
         isExternal sys (mid_to (msg_id (tmsg_msg rsout))) = true ->
-        Atomic rqin (IlblOuts (Some hdl) (rsout :: nil) :: hst)
+        Atomic (buildTInfo tid rqin)
+               (IlblOuts (Some (toTMsgU rqin)) (rsout :: nil) :: nil)
+               nil (Some rsout)
+  | AtomicCont:
+      forall ti hst mouts hdl houts,
+        Atomic ti hst mouts None ->
+        In hdl mouts ->
+        ForallMP (fun tmsg => isInternal sys (mid_to (msg_id (tmsg_msg tmsg))) = true) houts ->
+        Atomic ti (IlblOuts (Some hdl) houts :: hst)
+               (distributeMsgs houts (removeOnce tmsg_dec hdl mouts)) None
+  | AtomicFin:
+      forall ti hst hdl rsout,
+        Atomic ti hst (hdl :: nil) None ->
+        isExternal sys (mid_to (msg_id (tmsg_msg rsout))) = true ->
+        Atomic ti (IlblOuts (Some hdl) (rsout :: nil) :: hst)
                nil (Some rsout).
 
   Inductive Transactional: History -> Prop :=
@@ -47,9 +50,8 @@ Section PerSystem.
         tin = IlblIn msg ->
         Transactional (tin :: nil)
   | TrsAtomic:
-      forall rqin hst mouts orsout,
-        Atomic rqin hst mouts orsout ->
-        hst <> nil ->
+      forall ti hst mouts orsout,
+        Atomic ti hst mouts orsout ->
         Transactional hst.
 
   Definition Sequential (hst: History) :=
