src/SerialFacts.v
@@ -1,47 +1,26 @@
 Require Import Bool List String Peano_dec.
 Require Import Common ListSupport FMap.
-Require Import Syntax Semantics SemFacts StepDet Serial.
+Require Import Syntax Semantics SemFacts StepDet Serial TrsInv.
 
 Require Import Omega.
+Require Import Program.Equality.
 
 Set Implicit Arguments.
 
-Lemma SubHistory_refl:
-  forall hst, SubHistory hst hst.
-Proof.
-  intros; exists nil; reflexivity.
-Qed.
-
-Lemma SubHistory_cons:
-  forall l hst, SubHistory hst (l :: hst).
-Proof.
-  intros; exists (l :: nil); reflexivity.
-Qed.
-
-Lemma SubHistory_In:
-  forall l hst1 hst2,
-    In l hst1 ->
-    SubHistory hst1 hst2 ->
-    In l hst2.
-Proof.
-  unfold SubHistory; intros.
-  destruct H0 as [nhsg ?]; subst.
-  apply in_or_app; auto.
-Qed.
-
 Lemma atomic_emptyILabel_not_in:
-  forall sys rqin hst mouts orsout,
-    Atomic sys rqin hst mouts orsout ->
+  forall sys ti hst mouts orsout,
+    Atomic sys ti hst mouts orsout ->
     ~ In emptyILabel hst.
 Proof.
-  induction 1; simpl; intros; [auto| |];
-    try (intro Hx; elim IHAtomic; destruct Hx;
-         [discriminate|assumption]).
+  induction 1; simpl; intros.
+  - intro Hx; destruct Hx; [discriminate|auto].
+  - intro Hx; elim IHAtomic; destruct Hx; [discriminate|assumption].
+  - intro Hx; elim IHAtomic; destruct Hx; [discriminate|assumption].
 Qed.
 
 Lemma atomic_iLblIn_not_in:
-  forall sys rqin hst mouts orsout,
-    Atomic sys rqin hst mouts orsout ->
+  forall sys ti hst mouts orsout,
+    Atomic sys ti hst mouts orsout ->
     forall msg,
       ~ In (IlblIn msg) hst.
 Proof.
@@ -51,76 +30,125 @@ Proof.
 Qed.
 
 Lemma atomic_preserved:
-  forall impl1 rqin hst mouts orsout,
-    Atomic impl1 rqin hst mouts orsout ->
+  forall impl1 ti hst mouts orsout,
+    Atomic impl1 ti hst mouts orsout ->
     forall impl2,
       indicesOf impl1 = indicesOf impl2 ->
-      Atomic impl2 rqin hst mouts orsout.
+      Atomic impl2 ti hst mouts orsout.
 Proof.
   induction 1; simpl; intros.
   - econstructor; eauto.
-    unfold isExternal in *.
-    rewrite H1 in H; assumption.
-  - constructor; auto.
-    + unfold isInternal in *.
-      rewrite H4 in H1; assumption.
-    + unfold isInternal in *.
-      rewrite H4 in H2; assumption.
-  - constructor; auto.
-    + unfold isInternal in *.
-      rewrite H2 in H0; assumption.
     + unfold isExternal in *.
-      rewrite H2 in H1; assumption.
+      rewrite H1 in H; assumption.
+    + unfold isExternal in *.
+      rewrite H1 in H0; assumption.
+  - econstructor; eauto.
+    unfold isInternal in *.
+    rewrite H2 in H1; assumption.
+  - econstructor; eauto.
+    unfold isExternal in *.
+    rewrite H1 in H0; assumption.
 Qed.
 
 Lemma atomic_rs_out_1:
-  forall sys rqin hdl rsout hst mouts orsout,
-    Atomic sys rqin (IlblOuts (Some hdl) (rsout :: nil) :: hst) mouts orsout ->
+  forall sys ti hdl rsout hst mouts orsout,
+    Atomic sys ti (IlblOuts (Some hdl) (rsout :: nil) :: hst) mouts orsout ->
     isExternal sys (mid_to (msg_id (tmsg_msg rsout))) = true ->
     mouts = nil /\ orsout = Some rsout.
 Proof.
-  intros; inv H.
-  - exfalso; inv H10.
-    eapply (internal_external_false _ _ H2 H0); eauto.
-  - auto.
+  intros; inv H; auto.
+  exfalso.
+  inv H9.
+  eapply internal_external_false; eauto.
 Qed.
 
 Lemma atomic_rs_out_2:
-  forall sys rqin hst mouts rsout,
-    Atomic sys rqin hst mouts (Some rsout) ->
+  forall sys ti hst mouts rsout,
+    Atomic sys ti hst mouts (Some rsout) ->
     hst <> nil /\
     isExternal sys (mid_to (msg_id (tmsg_msg rsout))) = true /\
     mouts = nil /\
     exists hdl hst', hst = (IlblOuts (Some hdl) (rsout :: nil) :: hst').
 Proof.
-  intros; inv H.
-  repeat split; eauto.
-  discriminate.
+  intros; inv H;
+    try (repeat split; eauto; discriminate).
 Qed.
 
-Lemma atomic_mouts_tinfo:
-  forall sys rqin hst mouts orsout,
-    Atomic sys rqin hst mouts orsout ->
-    forall st1 st2,
-      steps_det sys st1 hst st2 ->
-      ForallMP (fun tmsg => tmsg_info tmsg = Some rqin) mouts.
-Proof.
-  induction 1; simpl; intros.
-  - constructor; auto.
-  - inv H4; apply ForallMP_distributeMsgs.
-    + eapply ForallMP_deqMP; eauto.
-    + inv H10.
-      remember (match tmsg_info fmsg with
-                | Some finfo => finfo
-                | None => {| tinfo_tid := nts; tinfo_rqin := tmsg_msg fmsg |}
-                end) as ntinfo; clear Heqntinfo.
-      specialize (IHAtomic _ _ H8).
-      eapply ForallMP_forall in IHAtomic; eauto.
-      simpl in IHAtomic; inv IHAtomic.
-      clear; induction (rule_outs _ _ _); [constructor|].
-      constructor; auto.
-  - constructor.
-Qed.
+(* Lemma atomic_tinfo: *)
+(*   forall sys ti hst mouts orsout, *)
+(*     Atomic sys ti hst mouts orsout -> *)
+(*     forall st1 st2, *)
+(*       steps_det sys st1 hst st2 -> *)
+(*       Forall (fun lbl => match lbl with *)
+(*                          | IlblOuts (Some hdl) _ => *)
+(*                            tmsg_info hdl = Some ti *)
+(*                          | _ => False *)
+(*                          end) hst /\ *)
+(*       ForallMP (fun tmsg => tmsg_info tmsg = Some ti) mouts. *)
+(* Proof. *)
+(*   induction 1; simpl; intros. *)
+(*   - discriminate. *)
+(*   - inv H3; inv H4. *)
+(*     destruct otid as [tid|]. *)
+(*     + destruct H0; [discriminate|inv H0]. *)
+(*       specialize (IHAtomic _ eq_refl _ _ H7); destruct IHAtomic. *)
+(*       inv H9. *)
+(*       split. *)
+(*       * eapply ForallMP_forall in H3; [|exact H1]. *)
+(*         eauto. *)
+(*       * apply ForallMP_distributeMsgs. *)
+(*         { eapply ForallMP_removeOnce; eauto. } *)
+(*         { clear; induction (rule_outs _ _ _); [constructor|]. *)
+(*           constructor; auto. *)
+(*         } *)
+(*     + inv H. *)
+(*       Common.dest_in. *)
+(*       split; auto. *)
+(*       unfold enqMP; rewrite app_nil_l. *)
+(*       unfold removeOnce. *)
+(*       destruct (tmsg_dec _ _); [|elim n; reflexivity]. *)
+(*       simpl. *)
+(*       inv H9. *)
+(*       clear; induction (rule_outs _ _ _); [constructor|]. *)
+(*       constructor; auto. *)
+
+(*   - split; [|constructor]. *)
+(*     inv H2; inv H3. *)
+(*     destruct otid as [tid|]. *)
+(*     + destruct H0; [discriminate|inv H0]. *)
+(*       specialize (IHAtomic _ eq_refl _ _ H6); destruct IHAtomic. *)
+(*       constructor; auto. *)
+(*     + inv H. *)
+(*       constructor; auto. *)
+(* Qed. *)
+
+(* Corollary atomic_hst_tinfo: *)
+(*   forall sys tid rqin hst mouts orsout, *)
+(*     Atomic sys (Some tid) rqin hst mouts orsout -> *)
+(*     forall st1 st2, *)
+(*       steps_det sys st1 hst st2 -> *)
+(*       Forall (fun lbl => match lbl with *)
+(*                          | IlblOuts (Some hdl) _ => *)
+(*                            tmsg_info hdl = Some (buildTInfo tid rqin) *)
+(*                          | _ => False *)
+(*                          end) hst. *)
+(* Proof. *)
+(*   intros. *)
+(*   eapply atomic_tinfo in H; eauto. *)
+(*   destruct H; auto. *)
+(* Qed. *)
+
+(* Corollary atomic_mouts_tinfo: *)
+(*   forall sys tid rqin hst mouts orsout, *)
+(*     Atomic sys (Some tid) rqin hst mouts orsout -> *)
+(*     forall st1 st2, *)
+(*       steps_det sys st1 hst st2 -> *)
+(*       ForallMP (fun tmsg => tmsg_info tmsg = Some (buildTInfo tid rqin)) mouts. *)
+(* Proof. *)
+(*   intros. *)
+(*   eapply atomic_tinfo in H; eauto. *)
+(*   destruct H; auto. *)
+(* Qed. *)
 
 Lemma trsMessages_app:
   forall ti mp1 mp2,
@@ -209,358 +237,23 @@ Proof.
     rewrite IHmp; reflexivity.
 Qed.
 
-Lemma msgs_tinfo_old':
-  forall sys sti ll st,
-    steps_det sys sti ll st ->
-    sti = getStateInit sys ->
-    ForallMP (fun tmsg =>
-                match tmsg_info tmsg with
-                | Some tinfo => tinfo_tid tinfo <= tst_tid st
-                | None => True
-                end) (tst_msgs st).
-Proof.
-  induction 1; simpl; intros; subst.
-  - cbn; constructor.
-  - specialize (IHsteps eq_refl).
-    inv H0; simpl.
-    + apply IHsteps; auto.
-    + apply ForallMP_enqMP; auto.
-      subst; cbn; auto.
-    + simpl in IHsteps.
-      apply ForallMP_distributeMsgs.
-      * destruct (tmsg_info fmsg) as [tinfo|].
-        { apply ForallMP_deqMP; auto. }
-        { apply ForallMP_deqMP.
-          apply ForallMP_forall; intros.
-          eapply ForallMP_forall in IHsteps; eauto.
-          destruct (tmsg_info msg); [omega|auto].
-        }
-      * apply firstMP_inMP in H5.
-        eapply ForallMP_forall in IHsteps; eauto.
-        destruct (tmsg_info fmsg) as [ftinfo|].
-        { clear -IHsteps Hts.
-          induction (rule_outs _ _ _); [constructor|].
-          simpl; find_if_inside; auto.
-          constructor; auto.
-        }
-        { clear.
-          induction (rule_outs _ _ _); [constructor|].
-          simpl; find_if_inside; auto.
-          constructor; auto.
-          simpl; omega.
-        }
-Qed.
-
-Lemma msgs_tinfo_old:
-  forall sys st,
-    Reachable steps_det sys st ->
-    ForallMP (fun tmsg =>
-                match tmsg_info tmsg with
-                | Some tinfo => tinfo_tid tinfo <= tst_tid st
-                | None => True
-                end) (tst_msgs st).
-Proof.
-  intros; inv H.
-  eapply msgs_tinfo_old'; eauto.
-Qed.
-
-Lemma external_msg_in_tinfo':
-  forall sys sti ll st,
-    steps_det sys sti ll st ->
-    sti = getStateInit sys ->
-    forall msgs,
-      msgs = tst_msgs st ->
-      forall tmsg,
-        InMP tmsg msgs ->
-        isExternal sys (mid_from (msg_id (tmsg_msg tmsg))) = true ->
-        tmsg_info tmsg = None.
-Proof.
-  induction 1; simpl; intros; subst; [inv H1|].
-  specialize (IHsteps eq_refl _ eq_refl).
-  inv H0; [eauto| |].
-
-  - simpl in H3.
-    apply inMP_enqMP_or in H3; destruct H3.
-    + subst; reflexivity.
-    + eapply IHsteps; eauto.
-
-  - simpl in H3.
-    apply inMP_distributeMsgs_or in H3; destruct H3.
-    + exfalso.
-      unfold intOuts in H0; apply filter_In in H0; destruct H0.
-      apply obj_in_sys_idx_internal in H1.
-      destruct H13.
-      clear -H0 H1 H3 H4.
-      induction (rule_outs _ _ _); [inv H0|].
-      inv H3; dest.
-      inv H0.
-      * simpl in H, H4.
-        unfold id in H; rewrite H in H4.
-        eapply internal_external_false; eauto.
-      * eapply IHl; eauto.
-    + eapply IHsteps; eauto.
-      simpl.
-      eapply inMP_deqMP; eauto.
-Qed.
-
-Lemma external_msg_in_tinfo:
-  forall sys st,
-    Reachable steps_det sys st ->
-    forall from to chn tmsg msgs,
-      msgs = tst_msgs st ->
-      firstMP from to chn msgs = Some tmsg ->
-      isExternal sys (mid_from (msg_id (tmsg_msg tmsg))) = true ->
-      tmsg_info tmsg = None.
-Proof.
-  intros; inv H.
-  eapply external_msg_in_tinfo'; eauto.
-  eapply firstMP_inMP; eauto.
-Qed.
-
-Lemma internal_msg_in_tinfo':
-  forall sys sti ll st,
-    steps_det sys sti ll st ->
-    sti = getStateInit sys ->
-    forall msgs,
-      msgs = tst_msgs st ->
-      forall tmsg,
-        InMP tmsg msgs ->
-        isInternal sys (mid_from (msg_id (tmsg_msg tmsg))) = true ->
-        exists tinfo, tmsg_info tmsg = Some tinfo.
-Proof.
-  induction 1; simpl; intros; subst; [inv H1|].
-  specialize (IHsteps eq_refl _ eq_refl).
-  inv H0; [eauto| |].
-
-  - simpl in H3.
-    apply inMP_enqMP_or in H3; destruct H3.
-    + exfalso; subst; simpl in *.
-      eauto using internal_external_false.
-    + eapply IHsteps; eauto.
-
-  - simpl in H3.
-    apply inMP_distributeMsgs_or in H3; destruct H3.
-    + clear -H0.
-      unfold intOuts in H0; apply filter_In in H0; destruct H0.
-      induction (rule_outs _ _ _); [inv H|].
-      inv H; auto.
-      simpl; eexists; reflexivity.
-    + eapply IHsteps; eauto.
-      simpl.
-      eapply inMP_deqMP; eauto.
-Qed.
-
-Lemma internal_msg_in_tinfo:
-  forall sys st,
-    Reachable steps_det sys st ->
-    forall from to chn tmsg msgs,
-      msgs = tst_msgs st ->
-      firstMP from to chn msgs = Some tmsg ->
-      isInternal sys (mid_from (msg_id (tmsg_msg tmsg))) = true ->
-      exists tinfo, tmsg_info tmsg = Some tinfo.
-Proof.
-  intros; inv H.
-  eapply internal_msg_in_tinfo'; eauto.
-  eapply firstMP_inMP; eauto.
-Qed.
-
-Lemma ts_monotone:
-  forall sys st1 lbl st2,
-    step_det sys st1 lbl st2 ->
-    tst_tid st1 <= tst_tid st2.
-Proof.
-  intros; inv H; auto.
-  simpl; destruct (tmsg_info fmsg); omega.
-Qed.
-
-Lemma reachable_hst_old':
-  forall sys hst sti st,
-    steps_det sys sti hst st ->
-    sti = getStateInit sys ->
-    Forall (fun tlbl =>
-              match tlbl with
-              | IlblOuts (Some hdl) _ =>
-                match tmsg_info hdl with
-                | Some tinfo => tinfo_tid tinfo <= tst_tid st
-                | None => True
-                end
-              | _ => True
-              end) hst.
-Proof.
-  induction 1; simpl; intros; subst; [constructor|].
-  constructor.
-  - assert (Reachable steps_det sys st2) by (econstructor; eauto).
-    apply msgs_tinfo_old in H1.
-    inv H0; simpl; auto.
-    simpl in H1.
-    apply firstMP_inMP in H6.
-    eapply ForallMP_forall in H1; eauto.
-    destruct (tmsg_info fmsg); auto.
-  - apply ts_monotone in H0.
-    specialize (IHsteps eq_refl).
-    clear -H0 IHsteps.
-    induction ll; simpl; intros; [constructor|].
-    inv IHsteps.
-    constructor; auto.
-    destruct a; auto.
-    destruct mhdl; auto.
-    destruct (tmsg_info t); auto.
-    omega.
-Qed.
-
-Lemma reachable_hst_old:
-  forall sys st1,
-    Reachable steps_det sys st1 ->
-    forall hst st2,
-      steps_det sys st1 hst st2 ->
-      Forall (fun tlbl =>
-                match tlbl with
-                | IlblOuts (Some hdl) _ =>
-                  match tmsg_info hdl with
-                  | Some tinfo => tinfo_tid tinfo <= tst_tid st2
-                  | None => True
-                  end
-                | _ => True
-                end) hst.
-Proof.
-  intros; inv H.
-  assert (steps_det sys (getStateInit sys) (hst ++ ll) st2).
-  { eapply steps_append; eauto. }
-  apply reachable_hst_old' in H; auto.
-  apply Forall_app_inv in H.
-  dest; auto.
-Qed.
+Definition AtomicOutsAInv (ti: TInfo)
+           (hst: History) (mouts: MessagePool TMsg) (ist: TState) :=
+  trsMessages ti (tst_msgs ist) = mouts.
 
 Lemma atomic_outs:
-  forall sys rqin hst mouts orsout,
-    Atomic sys rqin hst mouts orsout ->
-    hst <> nil ->
-    forall st1,
-      Reachable steps_det sys st1 ->
-      forall st2,
-        steps_det sys st1 hst st2 ->
-        trsMessages rqin (tst_msgs st2) = mouts.
+  forall sys, TrsAInv sys ValidTidState AtomicOutsAInv.
 Proof.
-  induction 1; simpl; intros; [intuition idtac| |].
-  - inv H6.
-    pose proof (atomic_mouts_tinfo H H10) as Htinfo.
-    eapply ForallMP_forall in Htinfo; eauto.
-    inv H12; simpl in *.
-    unfold distributeMsgs.
-    rewrite trsMessages_app.
-    destruct hst as [|lbl hst].
+Admitted.
 
-    + inv H10.
-      clear IHAtomic; inv H.
-      unfold InMP in H0; Common.dest_in.
-      unfold toTMsg in H; cbn in H; inv H.
-      eapply external_msg_in_tinfo in H14; eauto.
-      rewrite H14 in *; clear H14.
-      inv H9.
-      f_equal.
-      
-      * pose proof (msgs_tinfo_old H5); simpl in H.
-        replace (deqMP from to chn
-                       (enqMP (toTMsg {| tinfo_tid := nts; tinfo_rqin := tmsg_msg fmsg |}
-                                      (tmsg_msg fmsg)) nil))
-          with (nil (A:= TMsg)).
-        { (* NOTE: better to extract lemmas? *)
-          clear -H Hts.
-          assert (trsMessages {| tinfo_tid := nts; tinfo_rqin := tmsg_msg fmsg |} oims = nil).
-          { induction oims; [reflexivity|].
-            inv H; simpl.
-            destruct (tmsg_info a); auto.
-            destruct (tinfo_dec _ _); auto.
-            subst; simpl in H2; omega.
-          }
-          pose proof (trsMessages_deqMP_SubList
-                        {| tinfo_tid := nts; tinfo_rqin := tmsg_msg fmsg |}
-                        fidx (obj_idx obj) fchn oims).
-          rewrite H0 in H1.
-          apply SubList_nil_inv in H1; auto.
-        }
-        { unfold deqMP, enqMP; simpl.
-          apply firstMP_ValidMsgId in H3.
-          rewrite <-H3; simpl.
-          destruct (msgAddr_dec _ _); [|elim n; reflexivity].
-          reflexivity.
-        }
-          
-      * replace (intOuts sys (toTMsgs {| tinfo_tid := nts; tinfo_rqin := tmsg_msg fmsg |}
-                                      (rule_outs frule os (msg_value (tmsg_msg fmsg)))))
-          with (toTMsgs {| tinfo_tid := nts; tinfo_rqin := tmsg_msg fmsg |}
-                        (rule_outs frule os (msg_value (tmsg_msg fmsg)))).
-        { apply trsMessages_toTMsg. }
-        { clear -H2.
-          induction (toTMsgs {| tinfo_tid := nts; tinfo_rqin := tmsg_msg fmsg |}
-                             (rule_outs frule os (msg_value (tmsg_msg fmsg))));
-            [reflexivity|].
-          inv H2; simpl; dest.
-          rewrite H1.
-          rewrite IHl at 1 by assumption; reflexivity.
-        }
-
-    + assert (exists tinfo, tmsg_info fmsg = Some tinfo).
-      { inv H5.
-        eapply internal_msg_in_tinfo; [| |eassumption|eassumption].
-        { econstructor; eapply steps_append; eauto. }
-        { reflexivity. }
-      }
-      destruct H6 as [tinfo ?]; rewrite H6 in *.
-      inv Htinfo.
-      assert (lbl :: hst <> nil) by discriminate.
-      specialize (IHAtomic H7 _ H5 _ H10); clear H7; subst.
-      apply trsMessages_In_tinfo in H0; inv H0.
-      f_equal.
-      * assert (from = fidx /\ to = obj_idx obj /\ chn = fchn).
-        { apply firstMP_ValidMsgId in H3; apply firstMP_ValidMsgId in H14.
-          unfold ValidMsgId in *; simpl in *.
-          rewrite H3 in H14; inv H14; auto.
-        }
-        dest; subst; simpl.
-        eapply trsMessages_deqMP_comm; eauto.
-      * rewrite intOuts_Forall by assumption.
-        apply trsMessages_toTMsg.
-
-  - inv H4.
-    pose proof (atomic_mouts_tinfo H H8) as Htinfo.
-    eapply ForallMP_forall in Htinfo; [|left; reflexivity].
-    inv H; [exfalso; eapply internal_external_false; eauto|].
-    assert (IlblOuts (Some hdl0) houts :: hst0 <> nil) by discriminate.
-    specialize (IHAtomic H _ H3 _ H8).
-    clear H H2.
-    inv H10; simpl in *.
-
-    assert (exists tinfo, tmsg_info fmsg = Some tinfo).
-    { inv H3.
-      eapply internal_msg_in_tinfo; [| |eassumption|eassumption].
-      { econstructor; eapply steps_append; eauto. }
-      { reflexivity. }
-    }
-    destruct H as [tinfo ?]; rewrite H in *.
-    inv Htinfo.
-
-    rewrite H2.
-    replace (intOuts sys (rsout :: nil)) with (nil (A:= TMsg))
-      by (simpl; rewrite external_not_internal by assumption; reflexivity).
-    unfold distributeMsgs; rewrite app_nil_r.
-
-    rewrite trsMessages_deqMP_comm with (tmsg:= fmsg); try assumption.
-    rewrite IHAtomic.
-    simpl.
-    apply firstMP_ValidMsgId in H16. inv H16.
-    destruct (msgAddr_dec _ _); [|elim n; reflexivity].
-    reflexivity.
-Qed.
-
-Corollary atomic_rs_out_trsMessages_nil:
-  forall sys rqin hst mouts rsout,
-    Atomic sys rqin hst mouts (Some rsout) ->
+Corollary atomic_outs_trsMessages_nil:
+  forall sys ti hst mouts rsout,
+    Atomic sys ti hst mouts (Some rsout) ->
     forall st1,
-      Reachable steps_det sys st1 ->
+      ValidTidState st1 ->
       forall st2,
         steps_det sys st1 hst st2 ->
-        trsMessages rqin (tst_msgs st2) = nil.
+        trsMessages ti (tst_msgs st2) = nil.
 Proof.
   intros.
   pose proof (atomic_rs_out_2 H); dest; subst.
