src/TrsInv.v
@@ -1,0 +1,50 @@
+Require Import Bool List String Peano_dec.
+Require Import Common FMap ListSupport Syntax Semantics StepDet SemFacts.
+Require Import Simulation Serial.
+
+Set Implicit Arguments.
+
+Section Impl.
+  Variable (impl: System).
+
+  Definition TrsInvInit (ginv: TState -> Prop) :=
+    ginv (getStateInit impl).
+
+  Definition TrsInv (ginv: TState -> Prop) :=
+    forall ist1,
+      ginv ist1 ->
+      forall ihst ist2,
+        trsSteps impl ist1 ihst ist2 ->
+        ginv ist2.
+
+  Definition TrsInvIn (ginv: TState -> Prop) :=
+    forall ist1,
+      ginv ist1 ->
+      forall imin ist2,
+        step_det impl ist1 (IlblIn imin) ist2 ->
+        ginv ist2.
+
+  Definition TrsInvAtomic (ginv: TState -> Prop) :=
+    forall ti hst mouts orsout,
+      Atomic impl ti hst mouts orsout ->
+      forall ist1,
+        ginv ist1 ->
+        forall ist2,
+          steps_det impl ist1 hst ist2 ->
+          ginv ist2.
+
+  Definition TrsAInvInit
+             (ainv: TInfo -> History -> MessagePool TMsg -> TState -> Prop) :=
+    forall ti tst, ainv ti nil (enqMP (toTMsgU (tinfo_rqin ti)) nil) tst.
+
+  Definition TrsAInv (ginv: TState -> Prop)
+             (ainv: TInfo -> History -> MessagePool TMsg -> TState -> Prop) :=
+    forall ti hst mouts orsout,
+      Atomic impl ti hst mouts orsout ->
+      forall ist1 ist2,
+        steps_det impl ist1 hst ist2 ->
+        ginv ist1 ->
+        ainv ti hst mouts ist2.
+
+End Impl.
+
